\documentclass{article}
\usepackage[pagebackref,letterpaper=true,colorlinks=true,pdfpagemode=none,urlcolor=blue,linkcolor=blue,citecolor=blue,pdfstartview=FitH]{hyperref}

\usepackage{amsmath,amsfonts}
\usepackage{graphicx}
\usepackage{color}


\usepackage{algorithm}
\usepackage[noend]{algpseudocode}


\setlength{\oddsidemargin}{0pt}
\setlength{\evensidemargin}{0pt}
\setlength{\textwidth}{6.0in}
\setlength{\topmargin}{0in}
\setlength{\textheight}{8.5in}


\setlength{\parindent}{0in}
\setlength{\parskip}{5px}

%\input{macrosblog}

%%%%%%%%% For wordpress conversion

\def\more{}

\newif\ifblog
\newif\iftex
\blogfalse
\textrue


\usepackage{ulem}
\def\em{\it}
\def\emph#1{\textit{#1}}

\def\image#1#2#3{\begin{center}\includegraphics[#1pt]{#3}\end{center}}

\let\hrefnosnap=\href

\newenvironment{btabular}[1]{\begin{tabular} {#1}}{\end{tabular}}

\newenvironment{red}{\color{red}}{}
\newenvironment{green}{\color{green}}{}
\newenvironment{blue}{\color{blue}}{}

%%%%%%%%% Typesetting shortcuts

\def\B{\{0,1\}}
\def\xor{\oplus}

\def\P{{\mathbb P}}
\def\E{{\mathbb E}}
\def\var{{\bf Var}}

\def\N{{\mathbb N}}
\def\Z{{\mathbb Z}}
\def\R{{\mathbb R}}
\def\C{{\mathbb C}}
\def\Q{{\mathbb Q}}
\def\eps{{\epsilon}}

\def\bz{{\bf z}}

\def\true{{\tt true}}
\def\false{{\tt false}}

%%%%%%%%% Theorems and proofs

\newtheorem{exercise}{Exercise}
\newtheorem{theorem}{Theorem}
\newtheorem{lemma}[theorem]{Lemma}
\newtheorem{definition}[theorem]{Definition}
\newtheorem{corollary}[theorem]{Corollary}
\newtheorem{proposition}[theorem]{Proposition}
\newtheorem{example}{Example}
\newtheorem{remark}[theorem]{Remark}
\newenvironment{proof}{\noindent {\sc Proof:}}{$\Box$} %\medskip} 
%%%%%%%%% I added
\newtheorem{assumption}{Assumption}
%%%%%%%%

\begin{document}
Consider ODE
%\begin{equation}\label{eq:01}
$$ -  u'' + u = x, \ \forall x\in (0,1), \ u(0) = u(1) = 0.$$
%\end{equation} 
Answer the following questions:
\begin{enumerate}
 \item Prove that 
 %$$u(x) = x - \frac{\exp(\frac{x-1}{\sqrt \epsilon}) -  \exp(- \frac{x +1}{\sqrt \epsilon})}{ 1 - \exp(-\frac{2}{\sqrt \epsilon})}$$
 $$u(x) = x - \frac{\exp{(x-1}) -  \exp{(- x -1)}}{ 1 - \exp(-2)}$$
 is the unique solution.
 \item Using upwind finite difference scheme, find out the matrix $L^{h}$ and vector $R^{h} f$, such that the numerical solution satisfies $L^{h} u^{h} = R^{h} f$.
\item Convert $L^{h} u^{h} = R^{h} f$ to Markovian Reward Process.
\item Write a pseudocode for value iteration.
\item Write a pseudocode for first visit Monte-Carlo method.
 \item Prove the consistency
 \item Prove the stability.
 \item Find convergence rate.
\end{enumerate}

Hint: 
\begin{enumerate}
\item The equation to solve is $u\in C^2(0,1) \cap C[0,1]$ satisfying $Lu = \hat f$, where
the differential operator is
$$ L u(x) = \left\{ 
\begin{array}
{ll}
- u''(x) + u(x), & 0<x<1\\
u(x), & x = 0
\end{array}
\right. 
\ \forall u \in C^2
$$
The source term is 
$$ \hat f (x) = \left\{
\begin{array}
{ll}
f(x), & 0<x<1\\
0, & x = 0,1
\end{array}
\right.
$$

Let $h = 1/n$. UFD is the same as CFD since there is no first order term, and UFD is to solve for $u\in \mathbb R^{n+1}$ from $L^h u = R^h \hat f$, where
$$L^h u = 
\begin{bmatrix}
u_0 \\
- r u_0 + s u_1 - t u_2\\
\vdots \\
-r u_{i-1} + s u_i - t u_{i+1}\\
\vdots\\
-r u_{n-2} + s u_{n-1} - t u_n\\
u_n
\end{bmatrix}•
\ \forall u\in \mathbb R^{n+1},
$$
with
$$r = 1/h^2, s = 2/h^2 +1, t = 1/h^2.$$
and
$$
R^h f = [ f(x_0),  f(x_1), \ldots, f(x_{n-1}), f(x_n)], \forall f\in C([0,1])
$$ 

\item One needs to show the following for the consistency: there exists $\alpha>0$ such that
$$\|L^h R^h v - R^h L v\|_\infty \le K h^\alpha, \forall v\in C^2(0,1) \cap C[0,1], \forall \hbox{ small } h.$$
If $i=0$, then
$$(L^h R^h v)_i = (R^h v)_0 = v(x_0) = 0,$$
while
$$(R^h L v)_i = L v(x_0) = v(x_0) = 0.$$
If $i=n$, then
$$(L^h R^h v)_i = (R^h v)_n = v(x_n) = 0,$$
while
$$(R^h L v)_i = L v(x_n) = v(x_n) = 0.$$
If $1\le i \le n-1$, then
$$(L^h R^h v)_i = - \delta_h\delta_{-h} v (x_i) + v(x_i)$$
while
$$
(R^h L v)_i = - v''(x_i) + v(x_i).$$
Therefore, Taylor theorem implies that
$$\|L^h R^h v - R^h L v\|_\infty \le K h^2, \forall v\in C^2(0,1) \cap C[0,1], \forall \hbox{ small } h.$$

\item One needs to show the following for the stability: there exists $K$ such that
$$\|v\|_\infty \le K \|L^h v\|_\infty, \forall v\in \mathbb R^{n+1}.$$
If $|v_0| = \|v\|_\infty$, then
$$\|L^h v\|_\infty \ge |(L^h v)_0| = |v_0| = \|v\|_\infty.$$
If $|v_n| = \|v\|_\infty$, then
$$\|L^h v\|_\infty \ge |(L^h v)_n| = |v_n| = \|v\|_\infty.$$
If $|v_i| = \|v\|_\infty$ for some $1\le i \le n-1$, then
$$\|L^h v\|_\infty \ge |(L^h v)_i| 
= |- r v_{i-1} + s v_i - t v_{i+1}|
\ge s|v_i| - r|v_{i-1}| - t|v_{i+1}|
\ge (s - r - t) |v_i| \ge |v_i| = \|v\|_\infty.$$

\item Let $u^h$ be the numerical solution.
$$
\begin{array}
{ll}
\|u^h - R^h u\|_\infty 
 & \le \|L^h (u^h - R^h u)\|_\infty \\
& = \|L^h u^h - L^h R^h u\|_\infty \\
 & = \|R^h \hat f - L^h R^h u\|_\infty\\
& = \|R^h L u - L^h R^h u\|_\infty = O(h^2).
\end{array}•
$$
\end{enumerate}


\end{document}
